X2.dfy
@@ -1,4 +1,4 @@
-//Xlone_Via_Map -> Xlone_Xlone_Clone
+  //Xlone_Via_Map -> Xlone_Xlone_Clone
 //Xlone_Xlone_xClone -> Xlone_All_Owners, Object.make(), putInside/putOutside, Xlone_All_Fields
 //Xlone_All_Owners -> Xlone_Via_Map
 //Xlone_All_Fields -> Xlone_Field_Map
@@ -10,39 +10,112 @@ method Xlone_Via_Map(a : Object, m' : Klon)
 
   requires m'.calid()
   requires m'.readyAll()
-  requires allMapOwnersThruKlownOK(m')
+  requires checkClownershipAllObjects(m')
   requires COK(a, m'.oHeap) //ties owners into OHEAP but not KLON MAP
   requires klonCanKV(m',a,a)  //hmm, interesting... technically not right but
+  //must be neither objectinKlown or ownersinKlown!!!!
 
   ensures  a in m.m.Keys
   ensures  m.from(m')
   ensures  m.calid()
-  ensures  m.ownersInKlown(a)
-  {
-  m := m';
+  ensures  m.objectInKlown(a)
 
+    {
   print "CALL Clone_Via_Map ", fmtobj(a), " m':", m', "\n";
 
   print "VARIANT CVM ", |(m'.oHeap - m'.m.Keys) - {a}|, " ", |a.AMFO|, " ", |(a.fields.Keys )|, " ", 20, "\n";
 
-  if (a in m.m.Keys){ //already cloned, return
-    b := m.m[a];
+  if (a in m'.m.Keys){ //already cloned, return
+    b := m'.m[a];
     print "RETN Clone_Via_Map already cloned ", fmtobj(a),  " m':", m', "\n";
     return;
   }
 
-  if (outside(a,m.o)) { //outside. so just map to itself
+  if (outside(a,m'.o)) { //outside. so just map to itself
     b := a;
+
+
+
+    ///////////////////////////////  WHOOP WHOOP DA SOUND OF DA POLICE
+  reveal m'.calid();           assert m'.calid();
+  reveal m'.calidObjects();    assert m'.calidObjects();
+  reveal m'.calidOK();         assert m'.calidOK();
+  reveal m'.calidMap();        assert m'.calidMap();
+  reveal m'.calidSheep();      assert m'.calidSheep();
+
+
+
+  assert m'.m.Keys <= m'.oHeap;
+  assert m'.readyAll();
+//  assert m.readyOK(a);
+
+  assert a in m'.oHeap;
+  assert a !in m'.m.Keys;
+  assert COK(a, m'.oHeap);
+  assert m'.readyAll();
+  assert a.Ready() by { reveal COK(); }
+  assert checkClownershipAllObjects(m');
+    ///////////////////////////////  WHOOP WHOOP DA SOUND DAT I MISS
+
+//kjx I thikn this is OK for now
+//but
+    m := Xlone_All_Owners(a, m');
+
+    if (a in m.m.Keys){ //already cloned, return
+      b := m.m[a];
+      print "RETN Clone_Via_Map already cloned2 ", fmtobj(a),  " m:", m, "\n";
+      return;
+  }
+
+    assert a !in m'.m.Keys;
+    assert (outside(a,m'.o));
+    Klon.AintNoSunshine(a,m');
+    assert a !in m'.m.Values;
+
+    ///////////////////////////////  WHOOP WHOOP DA SOUND OF DA POLICE
+    assert m.from(m');
+
+    var k := a;
+    assert m.calid();
+    reveal m.calid(), m.calidObjects(), m.calidOK(), m.calidMap(), m.calidSheep(), m.AreWeNotMen();
+    reveal m.AreWeNotMen();
+    assert klonVMapOK(m.m);
+    assert m.readyAll();
+    assert checkClownershipAllObjects(m);
+    assert canVMapKV(m.m,k,k);
+    assert klonCanKV(m,k,k);
+    assert m.AreWeNotMen(k, m);//*
+    assert m.AreWeNotMen(k, klonKV(m,k,k));//*
+    assert m.ownersInKlown(k);
+    assert k  in m.oHeap;
+    assert k !in m.m.Keys;
+    assert k !in m.m.Values;
+    assert COK(k, m.oHeap);
+    assert m.m.Keys <= m.oHeap;
+        assert k.allExternalOwners() <= m.m.Keys;
+      assert outside(k, m.o);
+//    assert canMapOwnersThruKlown(k, klonKV(m,k,k));
+    assert canKlown(m, k, k,  klonKV(m,k,k));
+    ///////////////////////////////  WHOOP WHOOP DA SOUND DAT I MISS
+
     m := m.putOutside(a);
     print "RETN Clone_Via_Map: outside ", fmtobj(a), "\n";
     return; // end outside case
   }
 
+  assert a !in m'.m.Keys;
+
+  assert m'.readyAll();
+  assert m'.ownersInKlown(a);
  //start of the Inside case  --- //m'.calid() && COK(a, m'.oHeap)
-  b, m := Xlone_Clone_Clone(a, m);
-  //end of inside case
+  b, m := Xlone_Clone_Clone(a, m');
 
   print "RETN Clone_Via_Map: ", fmtobj(a), " pivot:", fmtobj(m.o), "\n";
+
+  assert  a in m.m.Keys;
+  assert  m.from(m');
+  assert  m.calid();
+  assert  m.objectInKlown(a);
 
 }//END Xlone_Via_Map
 
@@ -58,73 +131,182 @@ lemma somewhatFUCKED(a : Object)
 method Xlone_Clone_Clone(a : Object, m' : Klon)
   returns (b : Object, m : Klon)
     decreases (m'.oHeap - m'.m.Keys + {a}), |a.AMFO|, |a.fields.Keys|, 15
-//this case
-  requires IAO: inside(a, m'.o)
-  requires ANK: a !in m'.m.Keys
-
-  //all Clone
-  requires MCL: m'.calid()
-  requires AOH: a in m'.oHeap
-  requires COH: COK(a, m'.oHeap)
-  requires MRK: m'.readyOK(a)
+  requires inside(a, m'.o)
+  requires a !in m'.m.Keys
+  requires m'.calid()
+  requires a in m'.oHeap
+  requires COK(a, m'.oHeap)
+  requires CallOK(m'.oHeap)
+  requires m'.ownersInKlown(a)
+  requires forall o <- m'.m.Keys :: o.Ready()
+  requires forall o <- m'.m.Keys :: m'.alternateObjectInKlown(o)
+  requires a.Ready()
+  requires m'.o.Ready()
+  requires m'.alternateObjectInKlown(m'.o)
   requires m'.readyAll()
 
-  //requires COK(a, m'.m.Keys+{a}) //KJXFUCKEDFRIDAY13TH
+  requires checkClownershipAllObjects(m')
+
+  requires m'.boundsNestingOK(a, m'.m.Keys+{a})
+//
+//   requires IAO: inside(a, m'.o)
+//   requires ANK: a !in m'.m.Keys
+//   requires MCL: m'.calid()
+//   requires AOH: a in m'.oHeap
+//   requires COH: COK(a, m'.oHeap)
+//   requires CallOK(m'.oHeap)
+//   requires m'.ownersInKlown(a)
+//   requires forall o <- m'.m.Keys :: o.Ready()
+//   requires forall o <- m'.m.Keys :: m'.alternateObjectInKlown(o)
+//   requires a.Ready()
+//   requires m'.o.Ready()
+//   requires m'.alternateObjectInKlown(m'.o)
+//   requires m'.readyAll()
+//
+//   requires checkClownershipAllObjects(m')
+//
+//   requires BNK: m'.boundsNestingOK(a, m'.m.Keys+{a})
+
+
+
+  //hmmm
+    // ensures  a in m.m.Keys
+    // ensures  m.from(m')
+    // ensures  m.calid()
+    // ensures  m.objectInKlown(a)
+  //mmh
+
+
+  //requires COK(a, m'.m.Keys+{a}) //NO! NO! NO! //KJXFUCKEDFRIDAY13TH
   //need to establish this at the end of this method I guess...
-  //notably if we get here, a had better be in the heap but  NOT in the Klon (yet)
+  //notably if we get here, a had better be in the heap but NOT in the Klon (yet)
+  //similarly... //  requires MRK: m'.readyOK(a) mustent require this!!!
+
 {
+// assert ((a in m'.oHeap) && (COK(a, m'.oHeap))) by { reveal AOH, COH; }
+// assert MCL2: m'.calid() by { reveal MCL; }
+// assert (inside(a, m'.o)) by { reveal IAO; }
+// assert (a !in m'.m.Keys) by { reveal ANK; }
+// assert m'.readyAll();
+// assert (m'.m.Keys <= m'.oHeap) by { reveal MCL; m'.calidObjectsFromCalid(); }
+assert (m'.m.Keys <= m'.oHeap) by {  m'.calidObjectsFromCalid(); }
+//
+// assert a.fields.Keys == old(a.fields.Keys);  //unchanged?
+//
+// assert m'.readyAll();
+// assert m'.boundsNestingOK(a, m'.m.Keys+{a}) by { reveal BNK; }
+// assert (a.Ready())  by { assert COK(a, m'.oHeap); RVfromCOK(a, m'.oHeap); assert a.Ready(); }
+// assert (m'.m.Keys <= m'.oHeap);
+// //assert m.readyOK(a) by { reveal MRK; }
+//
+//  assert  a.AMFX == flattenAMFOs(a.owner);
+//  assert  a.AMFB == flattenAMFOs(a.bound);
+//
+//   print "CALL Clone_Clone_CLone of:", fmtobj(a), " owned by ", fmtown(a.owner) ,"\n";
+//   print "VARIANT CCC ", |(m'.oHeap - m'.m.Keys + {a})|, " ", |a.AMFO|, " ", |(a.fields.Keys)|, " ", 15, "\n";
+//
+//   print "Clone_Clone_Clone ", fmtobj(a), " calling CAO", fmtown(a.owner) ,"\n";
+//   printklon(m');
+// //   printmapping(m.m);
+// //  printobj(m.o);
+//
+// assert (m'.m.Keys <= m'.oHeap);
+// //assert m.readyOK(a);  //NO NO NO NO NO!
+//
+//   assert  m'.ownersInKlown(a);
+//
+// ///////////////////////////// SOUND OF THE PRE_CONDITIONS
+  assert m'.calid();// by { reveal MCL; }
+  assert m'.m.Keys <= m'.oHeap;
+  assert m'.readyAll();
+  assert a in m'.oHeap;
+  assert a !in m'.m.Keys;
+  assert COK(a, m'.oHeap);
+  // assert CCAO: checkClownershipAllObjects(m');
 
-assert ((a in m'.oHeap) && (COK(a, m'.oHeap))) by { reveal AOH, COH; }
-assert m'.calid() by { reveal MCL; }
-assert (inside(a, m'.o)) by { reveal IAO; }
-assert (a !in m'.m.Keys) by { reveal ANK; }
-assert BNK: m'.boundsNestingOK(a, m'.m.Keys+{a}) by { reveal MRK; assert m'.readyOK(a); m'.boundsNestingFromCalid(a, m'.m.Keys+{a}); }
-assert (m'.m.Keys <= m'.oHeap) by { reveal MCL; m'.calidObjectsFromCalid(); }
+  assert forall o <- m'.m.Keys :: o.Ready();
+  assert forall o <- m'.m.Keys :: m'.alternateObjectInKlown(o);
+  assert checkClownershipAllObjects(m');
+  assert a.Ready();
+// ////////////////////////////////////////////////////////////////////////////////
+  // assert a !in m'.m.Keys by { reveal ANK; }
+  // assert a  in m'.oHeap by { reveal AOH; }
+  // assert ((m'.oHeap - m'.m.Keys + {a}) >= (m'.oHeap - m'.m.Keys));
+  // assert (15 decreases to 12);
+  // assert (|a.fields.Keys|, 15 decreases to |a.fields.Keys|, 12);
+  // assert (|a.AMFO|, |a.fields.Keys|, 15
+  //   decreases to |a.AMFO|, |a.fields.Keys|, 12);
 
-m := m';
-assert m.from(m');
-     assert m'.boundsNestingOK(a, m'.m.Keys+{a}) by { reveal BNK; }
-assert (a.Ready())  by { assert COK(a, m'.oHeap); RVfromCOK(a, m'.oHeap); assert a.Ready(); }
-assert (m.m.Keys <= m.oHeap);
-assert m.readyOK(a) by { reveal MRK; }
+  // if ((m'.oHeap - m'.m.Keys + {a}) > (m'.oHeap - m'.m.Keys))
+  //   { assert ((m'.oHeap - m'.m.Keys + {a}), |a.AMFO|, |a.fields.Keys|, 15
+  //       decreases to (m'.oHeap - m'.m.Keys), |a.AMFO|, |a.fields.Keys|, 12); }
+  //  else
+  //   { assert ((m'.oHeap - m'.m.Keys + {a}) == (m'.oHeap - m'.m.Keys));
+  //     assert ((m'.oHeap - m'.m.Keys + {a}), |a.AMFO|, |a.fields.Keys|, 15
+  //       decreases to (m'.oHeap - m'.m.Keys), |a.AMFO|, |a.fields.Keys|, 12); }
 
- assert  a.AMFX == flattenAMFOs(a.owner);
- assert  a.AMFB == flattenAMFOs(a.bound);
+assert a !in m'.m.Keys;
+assert a  in m'.oHeap;
 
-  print "CALL Clone_Clone_CLone of:", fmtobj(a), " owned by ", fmtown(a.owner) ,"\n";
-  print "VARIANT CCC ", |(m'.oHeap - m'.m.Keys - {a})|, " ", |a.AMFO|, " ", |(a.fields.Keys)|, " ", 15, "\n";
+XCC_decreasesto_XAO(m',a);
 
-  print "Clone_Clone_Clone ", fmtobj(a), " calling CAO", fmtown(a.owner) ,"\n";
-  printmapping(m.m);
-
-  var aKeys := a.fields.Keys;
-
-assert ((m'.oHeap - m'.m.Keys), |a.AMFO|, |aKeys|, 15
-   decreases to (m.oHeap - m.m.Keys), |a.AMFO|, |a.fields.Keys|, 12);
-
-assert (m.m.Keys <= m.oHeap);
-assert m.readyOK(a);
+label B41:
+  assert m'.boundsNestingOK(a, m'.m.Keys+{a});
+  assert COK(a, m'.m.Keys+{a});
+  assert a.Ready();
+//  label B41:
+  var rm := Xlone_All_Owners(a, m');
 /////////////////////////////////////////////////////////////////////////////////
-  var rm := Xlone_All_Owners(a, m);
-/////////////////////////////////////////////////////////////////////////////////
 
-assert rm.from(m);
+assert old@B41(a.fields) == a.fields;
+assert old@B41(a.fieldModes) == a.fieldModes;
 
- var rowner := a.owner;
- var rbound := a.bound;
+  assert rm.from(m');
 
- assert ownerInsideOwner(rowner,rbound) by { reveal MRK; assert m'.readyOK(a); assert a.Ready(); assert a.owner >= a.bound; }
+  assert (m'.m.Keys+{a}) <= (rm.m.Keys+{a});
+  rm.boundsNestingWiderContext(a, (m'.m.Keys+{a}), (rm.m.Keys+{a}));
+
+  assert old@B41(m'.boundsNestingOK(a, m'.m.Keys+{a}));
+  assert old@B41(COK(a, m'.m.Keys+{a}));
+  assert old@B41(a.Ready());
+
+
+  assert (m'.m.Keys+{a}) <= (rm.m.Keys+{a});
+  rm.boundsNestingWiderContext(a, (m'.m.Keys+{a}), (rm.m.Keys+{a}));
+
+  assert m'.boundsNestingOK(a, m'.m.Keys+{a});
+  assert COK(a, m'.m.Keys+{a});
+  assert a.Ready();
+
+//  assert m'.boundsNestingOK(a, m'.m.Keys+{a}) by { reveal BNK; }
+//   rm.boundsNestingFromKlon(a, m'.m.Keys+{a}, m');
+  assert rm.boundsNestingOK(a, rm.m.Keys+{a});
+
+  assert rm.readyAll();
+  assert rm.ownersInKlown(a);
+  assert checkClownershipAllObjects(m');
+  assert a.fields.Keys == old(a.fields.Keys);  //unchanged?Q
+
+//REALLY MUST FIX!!!!!
+//REALLY MUST FIX!!!!!
+ var rowner := calculateClownership(a.owner, rm);
+ var rbound := rowner;
+ //REALLY MUST FIX!!!!!
+//REALLY MUST FIX!!!!!
+
+
+ assert ownerInsideOwner(rowner,rbound); // by { reveal MRK; assert m'.readyOK(a); assert a.Ready(); assert a.owner >= a.bound; }
 
  if (a in rm.m.Keys) {
 
     m := rm;
     b := m.at(a); //HMM
 
+      assert m.from(rm);
+      assert m.readyAll();
 
-assert m.from(rm);
-//END FUCKOFF
+    //END FUCKOFF
     print "RETN Clone_Clone_CLone ", fmtobj(a), " already cloned: abandoning ship!!\n";
-
 
     return;
   } // a in rm.m.Keys - i.e. randomly done while cloning owners
@@ -139,21 +321,48 @@ print "Clone_Clone_Clone ", fmtobj(a), " boodle boodle boodle\n";
 
 
   var context := rrm.oHeap+rrm.ns;    ///why haul ns in here??? --- cos this the owners for the clone!  - the clowners!
-     assert m'.boundsNestingOK(a, m'.m.Keys+{a}) by { reveal BNK; }
+//  assert m'.boundsNestingOK(a, m'.m.Keys+{a});  //or look in rrm
 
 print "CALLING MAKE...";
 
-  b := new Object.make(a.fieldModes, rowner, rrm.oHeap+rrm.ns, "clone of " + a.nick, rbound);
+assert COK(a, rrm.oHeap);
+COKowner(a, rrm.oHeap);
+assert CallOK(a.owner, rrm.oHeap);
+CallOKWiderContext2(a.owner, rrm.oHeap, context);
+assert CallOK(rowner, context);
+//HACKassert CallOK(context);
+b := new Object.make(a.fieldModes, rowner, rrm.oHeap+rrm.ns, "clone of " + a.nick, rbound);
 print "BACK FROM MAKE with ",fmtobj(b),"\n";
 
-assert CHAIN: b.AMFO  > b.AMFX >= b.AMFB == flattenAMFOs(rbound) >= rbound;
+assert a.fields.Keys == old(a.fields.Keys);  //unchanged?
 
+
+
+//OK at Sat 12 April 11am
+  assert  rm.boundsNestingOK(a,  rm.m.Keys+{a});
+  assert rrm.boundsNestingOK(a, rrm.m.Keys+{a});
+
+
+
+assert COK(b,rrm.oHeap+rrm.ns+{b});
+assert CHAIN: b.AMFO  > b.AMFX >= b.AMFB == flattenAMFOs(rbound) >= rbound;
 assert rrm.from(m');
+assert rrm.readyAll();
 assert rrm.calid();
 
+
+// assert (rrm.m.Keys+{a} ) == (m'.m.Keys+{a});
+// assert (m'.m.Keys+{a})  == old(m'.m.Keys+{a});
+
+//rrm.boundsNestingFromKlon(a,rrm.m.Keys+{a}, m');
+
+assert rrm.boundsNestingOK(a, rrm.m.Keys+{a});// by { reveal BNK; }
+
+
+
 //€€€€€€€€€€€€€€€€€€€€€€€€€€€€€€€€€€€€€€€€€€€€€€€€€€€€€€€€€€€€€€€€€€€€€€€
 //€€€€€€€€€€€€€€€€€€€€€€€€€€€€€€€€€€€€€€€€€€€€€€€€€€€€€€€€€€€€€€€€€€€€€€€
-//€€€€€€€€€€€€€€€€€€€€€€€€€€€€€€€€€€€€€€€€€€€€€€€€€€€€€€€€€€€€€€€€€€€€€€€
+//€€€€€€€€€€€€€€€€€€€€€€€€€€€€€€€€€€€€€€€€€€€€€€€€€€€€€€€€€€€€€€€€€€€€€€
 
 assert klonCanKV(rrm, a, b) by {
 
@@ -161,19 +370,18 @@ assert klonCanKV(rrm, a, b) by {
   var k  := a;
   var v  := b;
 
-     assert m'.boundsNestingOK(a, m'.m.Keys+{a}) by { reveal BNK; }
-     assert m'.boundsNestingOK(k, m'.m.Keys+{k}) by { reveal BNK; }
-
+     assert m'.boundsNestingOK(a, m'.m.Keys+{a});// by { reveal BNK; }
+     assert m'.boundsNestingOK(k, m'.m.Keys+{k});// by { reveal BNK; }
 
 //klonCanKV unpacked:
   assert klonVMapOK(c'.m) by { KlonVMapOKfromCalid(c'); }
   assert canVMapKV(c'.m, k, v);
-  assert (k in c'.oHeap) by { reveal AOH; }
+  assert (k in c'.oHeap);// by { reveal AOH; }
   assert (if (v==k) then (v in c'.oHeap) else (v !in c'.oHeap));
   assert c'.boundsNestingOK(k, c'.oHeap) by { c'.boundsNestingFromCalid(k, c'.oHeap); } //GRRR
   assert c'.boundsNestingOK(v, c'.oHeap+c'.ns+{v})  by { c'.boundsNestingFromCalid(v, c'.oHeap+c'.ns+{v}); }
-  assert m'.boundsNestingOK(k, m'.m.Keys+{k}) by { reveal BNK; }
-  assert c'.boundsNestingOK(k, c'.m.Keys+{k}) by { reveal BNK;
+  assert m'.boundsNestingOK(k, m'.m.Keys+{k});// by { reveal BNK; }
+  assert c'.boundsNestingOK(k, c'.m.Keys+{k}) by { //reveal BNK;
                                                    assert m'.boundsNestingOK(k, m'.m.Keys+{k});
                                                    m'.boundsNestingWiderContext(k, m'.m.Keys+{k}, c'.m.Keys+{k});
                                                    c'.boundsNestingFromCalid(k, c'.m.Keys+{k});  }
@@ -184,15 +392,114 @@ assert klonCanKV(rrm, a, b) by {
 //€€€€€€€€€€€€€€€€€€€€€€€€€€€€€€€€€€€€€€€€€€€€€€€€€€€€€€€€€€€€€€€€€€€€€€€
 //€€€€€€€€€€€€€€€€€€€€€€€€€€€€€€€€€€€€€€€€€€€€€€€€€€€€€€€€€€€€€€€€€€€€€€€
 //€€€€€€€€€€€€€€€€€€€€€€€€€€€€€€€€€€€€€€€€€€€€€€€€€€€€€€€€€€€€€€€€€€€€€€€
+//Hollywookd Fantasie
 
-assert klonCanKV(rrm, a, b);
+  assert klonCanKV(rrm, a, b);
 
-    var km := klonKV(rrm,a,b); //there it go4s in!
-    var xm := km;
+  var xm := klonKV(rrm,a,b); //there it go4s in!
+
+  assert forall oo <- rrm.m.Keys :: rrm.readyOK(oo);
+  assert a.Ready();
+  assert rrm.ownersInKlown(a);
+  forall oo <- xm.m.Keys ensures (xm.readyOK(oo)) //by jjj
+   {
+      if (oo in rrm.m.Keys)
+        { assert rrm.readyOK(oo); }
+        else
+        { assert (oo == a) && (xm.readyOK(a)); }
+   }
+  assert forall oo <- xm.m.Keys :: xm.readyOK(oo);
+
+
+  assert xm.oxtra  == rrm.oxtra;
+  assert xm.cxtra  == rrm.cxtra;
+  assert xm.o_amfx <= xm.m.Keys;
+  assert xm.c_amfx == rrm.c_amfx;
+
+  assert xm.o_amfx == rrm.o_amfx <= rrm.m.Keys <= xm.m.Keys;
+
+  var mx := mapThruKlon(xm.o_amfx,  xm);
+  var mr := mapThruKlon(rrm.o_amfx, rrm);
+  // var mxr := (mx == mr);
+  // assert mxr;
+  // print "XXX FUCKER ", mxr, "\n";
+  // print "XXX FUCKER ", fmtown(mx), "\n";
+  // print "XXX FUCKER ", fmtown(mr), "\n";
+  // assert mapThruKlon(xm.o_amfx, xm) == mapThruKlon(rrm.o_amfx, rrm);
+
+///FOOKING HELL
+  assert rrm.readyAll();
+  assert xm.from(rrm);
+
+  assert (xm.o_amfx <= xm.m.Keys);
+  // assert (xm.oxtra == mapThruKlon(xm.o_amfx, xm) - xm.c_amfx);
+  // assert (xm.cxtra == xm.c_amfx - mapThruKlon(xm.o_amfx, xm));
+  assert (forall k <- xm.m.Keys :: xm.readyOK(k));
+
+  assert xm.readyAll();
+
+//  assert  rrm.readyOK(a);
+//  assert  forall o <- rrm.m.Keys :: rrm.readyOK(o);
+//  assert  allMapOwnersThruKlownOK(rrm);
+  assert  klonAllOwnersAreCompatible(rrm) by {
+       assert rrm.calid();
+       reveal rrm.calid();
+       assert rrm.calidMap();
+       reveal rrm.calidMap();
+       assert  klonAllOwnersAreCompatible(rrm);
+  }
+  assert  rrm.calid();
+  assert  MFUCKING: rrm.calid();
+  assert  klonVMapOK(rrm.m);
+  assert  klonCanKV(rrm, a, b);
+  assert  a in rrm.oHeap;
+  assert  COK(a, rrm.oHeap);
+  assert  (b==a) ==> (b in rrm.oHeap);
+  assert  (b==a) ==> (COK(b,rrm.oHeap));
+  assert  (b!=a) ==> (COK(b,rrm.oHeap+rrm.ns+{b}));
+  assert  (b!=a) ==> b in xm.ns;
+  assert  a.Ready();
+  assert  xm == klonKV(rrm, a, b);
+  assert  mapGEQ(xm.m, rrm.m);
+  assert  klonLEQ(rrm, xm);
+  assert  (b==a) == (outside(a, rrm.o));
+  assert  (b!=a) ==> (b.fields == map[]);
+
+  assert forall o <- xm.m.Keys :: o.Ready();
+  assert forall o <- xm.m.Keys :: xm.alternateObjectInKlown(o);
+  assert xm.readyAll();
+  assert forall o <- xm.m.Keys :: checkClownership(o,m);
+  assert checkClownershipAllObjects(xm);
+  assert forall o <- xm.m.Keys :: xm.readyOK(o);
+///FOOKING
+
+  klonCalidKVCalid(rrm,                                                                                                                                                                                                                       a,b,xm);
+
+
+  assert xm.from(rrm);
+
+  assert xm.calid() by {
+
+  assert
+    && xm.o in xm.oHeap
+    && xm.m.Keys <= xm.oHeap
+    && xm.ns !! xm.oHeap
+    && xm.m.Values <= xm.ns + xm.oHeap
+    && xm.ns <= xm.m.Values
+    ;
+
+
+  reveal xm.calidObjects();    assert xm.calidObjects();
+  reveal xm.calidOK();         assert xm.calidOK();
+  reveal xm.calidMap();        assert xm.calidMap();
+  reveal xm.calidSheep();      assert xm.calidSheep();
+  reveal xm.calid();           assert xm.calid();
+}
+
 
   //  var km := rrm.(ns := rrm.ns + nu(a,b)).(m:= VMapKV(rrm.m,a,b));
 
-print "go4s: ", |km.m|, " ns: ", |km.ns|,"\n";
+print "go4s: ", |xm.m|, " ns: ", |xm.ns|,"\n";
 
 var amxo := flattenAMFOs(a.owner);
 
@@ -203,7 +510,7 @@ var amxo := flattenAMFOs(a.owner);
 
   print "Clone_Clone_Clone map updated ", fmtobj(a), ":=", fmtobj(b) ,"\n";
 
-//COK(a, mmKeys) can only be establshed there
+
 
 
 //££££££££££££££££££££££££££££££££££££££££££££££4£££££££££££££££££££££££££££££££££££££££££££££££££££££££££££££
@@ -251,6 +558,18 @@ assert (
 
 
 //££££££££££££££££££££££££££££££££££££££££££££££££££££££££££££££££££££££££££££££££££££££££££££££££££££££££££
+  assert xm.calid();
+  assert xm.readyAll();
+  assert xm.readyOK(a);
+  assert xm.objectInKlown(a);
+  assert checkClownershipAllObjects(xm);
+  assert COK(a, xm.oHeap);
+  assert xm.m.Keys <= xm.oHeap;
+  assert b.fields.Keys == {};
+  assert b in xm.m.Values;
+  assert b in xm.ns;
+  assert a.fieldModes == b.fieldModes;
+//€€€€€€€€€€€€€€€€€€€€€€€€€€€€€€€€€€€€€€€€€€€€€€€€€€@x
 
    m := Xlone_All_Fields(a,b, xm);
 
@@ -287,11 +606,17 @@ method Xlone_All_Owners(a : Object,  m' : Klon)  returns (m : Klon)
   requires m'.calid()
   requires m'.m.Keys <= m'.oHeap   //calid via calidObjects...
   requires m'.readyAll()
-  requires m'.readyOK(a)
+//  requires m'.readyOK(a)
 
   requires a in m'.oHeap
   requires a !in m'.m.Keys //mustn't have cloned a yet...
   requires COK(a, m'.oHeap)
+
+  requires forall o <- m'.m.Keys :: o.Ready()
+  requires forall o <- m'.m.Keys :: m'.alternateObjectInKlown(o)
+
+  requires CCAO: checkClownershipAllObjects(m')
+  requires       checkClownershipAllObjects(m')
 
 
 //  requires m'.readyAll()
@@ -302,11 +627,21 @@ method Xlone_All_Owners(a : Object,  m' : Klon)  returns (m : Klon)
 
   ensures  m.ownersInKlown(a)
 
+  ensures  m.readyAll()
+
 //probably redundant versions
   ensures a.owner <= m.m.Keys
   ensures a.allExternalOwners() <= m.m.Keys
   ensures mapThruKlon(a.allExternalOwners(),m) <= m.m.Values
 //end   redundant versions
+  ensures  forall o <- m.m.Keys :: o.Ready()
+  ensures  forall o <- m.m.Keys :: m.alternateObjectInKlown(o)
+  ensures  m.readyAll()
+  ensures  checkClownershipAllObjects(m)
+
+  ensures unchanged(a`fields, a`fieldModes)
+  ensures old(a.fields) == a.fields
+  ensures old(a.fieldModes) == a.fieldModes
   modifies {}
 {
   print "CALL Clone_All_Owner of:", fmtobj(a), " owned by ", fmtown(a.owner) ,"\n";
@@ -318,6 +653,8 @@ method Xlone_All_Owners(a : Object,  m' : Klon)  returns (m : Klon)
   assert rm.m.Keys <= rm.oHeap;
   assert a in rm.oHeap;
   assert COK(a, rm.oHeap);
+  assert checkClownershipAllObjects(rm) by { reveal CCAO; }
+  assert CCAO_1: checkClownershipAllObjects(rm);
 
 
   var b : Object;  //do we care..
@@ -328,6 +665,8 @@ method Xlone_All_Owners(a : Object,  m' : Klon)  returns (m : Klon)
   assert xm.m.Keys <= xm.oHeap;
   assert a in xm.oHeap;
   assert COK(a, xm.oHeap);
+  assert         checkClownershipAllObjects(xm) by { reveal CCAO_1; }
+  assert CCAO_2: checkClownershipAllObjects(xm);
 
   var xo : Object;
   var rr : Object;
@@ -350,6 +689,7 @@ method Xlone_All_Owners(a : Object,  m' : Klon)  returns (m : Klon)
     assert CallOK(xm.oHeap);
     assert MX <= xm.oHeap;
 
+  assert checkClownershipAllObjects(xm);
 
      print "PRELOOP ", |MX|," a in Keys ", (a !in xm.m.Keys), "\n";
 
@@ -365,6 +705,7 @@ method Xlone_All_Owners(a : Object,  m' : Klon)  returns (m : Klon)
     invariant xm.from(m')
     invariant MX <= xm.oHeap
     invariant CallOK(xm.oHeap)
+    invariant xm.readyAll()
     invariant a.owner - {a} <= xm.m.Keys + MX //this one?
     invariant a.owner <= a.AMFO
     invariant oldmok ==> assigned(oldmks)
@@ -373,6 +714,8 @@ method Xlone_All_Owners(a : Object,  m' : Klon)  returns (m : Klon)
     invariant oldmok ==> ((m'.oHeap - oldmks) > (xm.oHeap - xm.m.Keys))
     invariant xm.m.Keys >= (m'.m.Keys)
     invariant xm.m.Values >= (m'.m.Values)
+    invariant checkClownershipAllObjects(xm)
+
   {
       print "LOOPTOP ", |MX|," a in Keys ", (a !in xm.m.Keys), "\n";
 
@@ -389,8 +732,11 @@ assert xo.Ready();
 
 //    assert xm.readyOK(xo);
 
+  assert checkClownershipAllObjects(xm);
+
     rr, rm := Xlone_Via_Map(xo, xm);
 
+  assert checkClownershipAllObjects(rm);
 assert rm.from(xm);
 
     if (a in rm.m.Keys) {
@@ -403,6 +749,7 @@ assert m.from(rm);  assert m.calid();
 
   assert  m.from(m');
   assert  m.ownersInKlown(a);
+  assert checkClownershipAllObjects(m);
 
       return;
     }  // if a is in m.Keys after clone -- if it got added magically...
@@ -413,8 +760,13 @@ assert m.from(rm);  assert m.calid();
     oldmks := xm.m.Keys;
     oldmok := true;
     xm := rm;
+    assert checkClownershipAllObjects(rm);
     assert xm.from(rm);
+    assert checkClownershipAllObjects(xm);
+
   } // end loop MX
+
+  assert checkClownershipAllObjects(xm);
 
   m := xm;
 assert m.from(xm);  assert m.calid();
@@ -424,6 +776,7 @@ assert m.from(xm);  assert m.calid();
 
   assert  m.from(m');
   assert  m.ownersInKlown(a);
+  assert checkClownershipAllObjects(m);
 }//END Xlone_All_Owners
 
 
@@ -448,10 +801,10 @@ method Xlone_All_Fields(a : Object, b : Object, m' : Klon)
   requires m'.calid()
   requires m'.readyAll()
   requires m'.readyOK(a)
-  requires m'.readyOK(a)
-  requires allMapOwnersThruKlownOK(m')
+  requires m'.objectInKlown(a)
+  requires checkClownershipAllObjects(m')
   requires COK(a, m'.oHeap)  //GRRR need to resolve WRT readyOK() and Valid()
-  requires klonCanKV(m',a,a)
+//  requires klonCanKV(m',a,a)
 
   requires m'.m.Keys <= m'.oHeap
   requires b.fields.Keys == {}
@@ -483,8 +836,10 @@ method Xlone_All_Fields(a : Object, b : Object, m' : Klon)
 
   assert m.calid();
   assert m.readyAll();
-  assert m.readyOK(a);
-  assert allMapOwnersThruKlownOK(m');
+//  assert m.readyOK(a);
+  assert m.objectInKlown(a);
+//  assert allMapOwnersThruKlownOK(m');
+assert checkClownershipAllObjects(m);
 
   assert COK(a, m'.oHeap);
   assert klonCanKV(m',a,a);
@@ -549,7 +904,8 @@ method Xlone_All_Fields(a : Object, b : Object, m' : Klon)
 
     invariant m.calid()
     invariant m.readyAll()
-    invariant m.readyOK(a)
+  //  invariant m.readyOK(a)
+    invariant m.objectInKlown(a)
 
     invariant ((m.oHeap - m.m.Keys +{a}) <= (m'.oHeap - m'.m.Keys +{a}))
     invariant ((m.oHeap - m.m.Keys) <= (m'.oHeap - m'.m.Keys))
@@ -599,8 +955,8 @@ assert (
 
   assert m.calid();
   assert m.readyAll();
-  assert m.readyOK(a);
-  assert allMapOwnersThruKlownOK(m);
+  assert m.objectInKlown(a);
+  assert checkClownershipAllObjects(m);
 
   assert COK(a, m'.oHeap);
   assert klonCanKV(m',a,a);
@@ -638,9 +994,15 @@ method Xlone_Field_Map(a : Object, n : string, b : Object, m' : Klon) returns (m
 
   requires m'.calid()
   requires m'.readyAll()
-  requires m'.readyOK(a)
+//  requires m'.readyOK(a)
+  requires a.Ready()
+  requires m'.objectInKlown(a)
 
-  requires allMapOwnersThruKlownOK(m')
+  requires forall o <- m'.m.Keys :: o.Ready()
+  requires forall o <- m'.m.Keys :: m'.alternateObjectInKlown(o)
+
+//  requires allMapOwnersThruKlownOK(m')
+  requires checkClownershipAllObjects(m')
   requires COK(a, m'.oHeap)
   requires klonCanKV(m',a,a)
 
@@ -658,7 +1020,7 @@ method Xlone_Field_Map(a : Object, n : string, b : Object, m' : Klon) returns (m
   ensures  m.calid()
   ensures  old(m'.calid())
   ensures  m.readyAll()
-  ensures  m.readyOK(a)
+  ensures  m.objectInKlown(a)
 
   ensures  unchanged(a)
   ensures  unchanged(m'.oHeap)
@@ -696,8 +1058,10 @@ method Xlone_Field_Map(a : Object, n : string, b : Object, m' : Klon) returns (m
 
   assert m.calid();
   assert m.readyAll();
-  assert m.readyOK(a);
-  assert allMapOwnersThruKlownOK(m);
+//  assert m.readyOK(a);
+assert m.objectInKlown(a);
+assert checkClownershipAllObjects(m);
+//  assert allMapOwnersThruKlownOK(m);
   assert COK(a, m.oHeap);
   assert klonCanKV(m,a,a);
 
@@ -726,8 +1090,10 @@ assert
 
   assert m.calid();
   assert m.readyAll();
-  assert m.readyOK(a);
-  assert allMapOwnersThruKlownOK(m);
+//  assert m.readyOK(a);
+assert m.objectInKlown(a);
+assert checkClownershipAllObjects(m);
+//  assert allMapOwnersThruKlownOK(m);
   assert COK(a, m.oHeap);
   assert klonCanKV(m,a,a);
 
@@ -781,3 +1147,17 @@ assert
 function fielddiff(a : Object, b : Object) : nat
   reads a, b
   {| a.fields.Keys - b.fields.Keys |}
+
+
+lemma XCC_decreasesto_XAO(m' : Klon, a : Object)
+  requires a !in m'.m.Keys
+  requires a  in m'.oHeap
+  ensures  ((m'.oHeap - m'.m.Keys + {a}), |a.AMFO|, |a.fields.Keys|, 15
+        decreases to (m'.oHeap - m'.m.Keys), |a.AMFO|, |a.fields.Keys|, 12)
+{
+  // assert (15 decreases to 12);
+  // assert (|a.fields.Keys|, 15 decreases to |a.fields.Keys|, 12);
+  // assert (|a.AMFO|, |a.fields.Keys|, 15
+  //   decreases to |a.AMFO|, |a.fields.Keys|, 12);
+  // assert ((m'.oHeap - m'.m.Keys + {a}) >= (m'.oHeap - m'.m.Keys));
+}
